ott/coq/Context.v
@@ -2,6 +2,9 @@ Require Import Bool List.
 
 Require Import Common.
 
+Definition add {A B} (E : list (A * B)) a b :=
+  (a, b) :: E.
+
 Inductive Lookup {A B : Type} : list (A * B) -> A -> B -> Type :=
   | Lookup_hd     a b E :                           Lookup (cons (a,b) E) a b
   | Lookup_tl x y a b E : x <> a -> Lookup E a b -> Lookup (cons (x,y) E) a b.
@@ -111,7 +114,7 @@ Proof.
     constructor 1.
   + eapply (Hdisjoint a').
     constructor 2; eassumption.
-Qed.
+Qed.  
 
 Lemma Disjoint_app {A B C} {eq_dec : DecidableEq A} {E1 E2 : list (A * B)} {E : list (A * C)}:
   Disjoint E1 E ->
@@ -126,4 +129,380 @@ Proof.
     eapply Disjoint_cons_left.
     + eassumption.
     + exact (IHE1 H H2).
+Qed.
+
+Definition context_ind {A B} (P : list (A * B) -> Type) :
+  (P nil) ->
+  (forall a b E, P E -> P (add E a b)) ->
+  (forall E, P E).
+Proof.
+  intros Hnil Hcons.
+  induction E as [|[? ?]].
+  + exact Hnil.
+  + eapply Hcons; assumption.
+Qed.
+
+
+Inductive linear {A B} : list (A * B) -> Type :=
+  | LinearNil        : linear nil
+  | LinearCons a b E : (forall b, neg (Lookup E a b)) -> linear E -> linear ((a, b) :: E).
+
+Fixpoint remove_var {A B} {eq_dec : DecidableEq A} a E : list (A * B) :=
+  match E with
+  | nil             => nil
+  | cons (a', b') E => match decide a a' : Decision (a = a') with
+                       | inl _ => (remove_var a E)
+                       | inr _ => (a', b') :: (remove_var a E)
+                       end
+  end.
+
+Fixpoint remove_var_fun {A B} (eq_fun : A -> A -> bool) a E : list (A * B) :=
+  match E with
+  | nil             => nil
+  | cons (a', b') E => if eq_fun a a' 
+                         then remove_var_fun eq_fun a E
+                         else (a', b') :: remove_var_fun eq_fun a E
+  end.
+
+Lemma remove_var_fun_complete {A B} (eq_fun : A -> A -> bool) a (E : list (A * B)) :
+  (forall x y, boolSpec (eq_fun x y) (x = y)) ->
+  forall a' b', 
+    neg (a = a') ->
+    Lookup E a' b' ->
+    Lookup (remove_var_fun eq_fun a E) a' b'.
+Proof.
+  intros eq_fun_correct.
+  induction E as [|[? ?] E IH]; simpl.
+  - inversion 2.
+  - inversion 2;
+    match goal with
+    | [|- context[eq_fun ?a1 ?a2]] =>
+        generalize (eq_fun_correct a1 a2);
+        destruct (eq_fun a1 a2)
+    end; my_auto.
+Qed.
+
+Lemma remove_var_complete {A B} {eq_dec : DecidableEq A} a (E : list (A * B)) :
+  forall a' b', 
+    neg (a = a') ->
+    Lookup E a' b' ->
+    Lookup (remove_var a E) a' b'.
+Proof. induction E; inversion 2; my_auto. Qed.
+
+Lemma remove_var_fun_sound {A B} (eq_fun : A -> A -> bool) a (E : list (A * B)) :
+  (forall x y, boolSpec (eq_fun x y) (x = y)) ->
+  forall a' b', 
+    neg (a = a') ->
+    Lookup (remove_var_fun eq_fun a E) a' b' ->
+    Lookup E a' b'.
+Proof.
+  intros eq_fun_correct ? ? ?.
+  induction E as [|[? ?] E IH]; simpl.
+  - inversion 1.
+  - match goal with
+    | [|- context[eq_fun ?a1 ?a2]] =>
+        generalize (eq_fun_correct a1 a2);
+        destruct (eq_fun a1 a2);
+        simpl
+    end.
+    + intros;      my_auto.
+    + inversion 2; my_auto.
+Qed.
+
+Lemma remove_var_sound {A B} {eq_dec : DecidableEq A} a (E : list (A * B)) :
+  forall a' b',
+    neg (a = a') ->
+    Lookup (remove_var a E) a' b' ->
+    Lookup E a' b'.
+Proof.
+  intros a' b' Hneq.
+  induction E as [| [a'' b'']]; simpl.
+  - inversion 1.
+  - decide_destruct;
+    inversion 1;
+    my_auto.
+Qed.
+
+Lemma remove_var_fun_Lookup {A B} (eq_fun : A -> A -> bool) a (E : list (A * B)) :
+  (forall x y, boolSpec (eq_fun x y) (x = y)) ->
+  forall b, neg (Lookup (remove_var_fun eq_fun a E) a b).
+Proof.
+  intros eq_fun_correct.
+  induction E as [|[? ?] E IH]; simpl.
+  - inversion 1.
+  - match goal with
+    | [|- context[eq_fun ?a1 ?a2]] =>
+        generalize (eq_fun_correct a1 a2);
+        destruct (eq_fun a1 a2);
+        simpl
+    end.
+    + my_auto.
+    + inversion 2.
+      * my_auto.
+      * firstorder.
+Qed.
+
+Lemma remove_var_Lookup {A B} {eq_dec : DecidableEq A} a (E : list (A * B)) :
+  forall b, neg (Lookup (remove_var a E) a b).
+Proof.
+  induction E as [| [? ?]]; simpl.
+  - inversion 1.
+  - destruct_decide.
+    + assumption.
+    + inversion 1; my_auto; firstorder.
+Qed.
+
+Fixpoint linearize {A B} {eq_dec : DecidableEq A} E : list (A * B) :=
+  match E with
+  | nil           => nil
+  | cons (a, b) E => cons (a, b) (remove_var a (linearize E))
+  end.
+
+Fixpoint linearize_fun {A B} (eq_fun : A -> A -> bool) E : list (A * B) :=
+  match E with
+  | nil           => nil
+  | cons (a, b) E => cons (a, b) (remove_var_fun eq_fun a (linearize_fun eq_fun E))
+  end.
+
+Lemma linearize_fun_sound {A B} {eq_fun : A -> A -> bool} (E : list (A * B)) :
+  (forall x y, boolSpec (eq_fun x y) (x = y)) ->
+  forall a' b',
+    Lookup (linearize_fun eq_fun E) a' b' ->
+    Lookup E a' b'.
+Proof.
+  intros eq_fun_correct.
+  induction E as [|[? ?]]; simpl.
+  - inversion 1.
+  - inversion 1; subst.
+    + constructor.
+    + constructor 2.
+      * assumption.
+      * apply IHE.
+        eapply remove_var_fun_sound; eassumption.
+Qed.
+
+Lemma linearize_sound {A B} {eq_dec : DecidableEq A} (E : list (A * B)) :
+  forall a' b',
+    Lookup (linearize E) a' b' ->
+    Lookup E a' b'.
+Proof.
+  induction E as [|[? ?]]; simpl.
+  - inversion 1.
+  - inversion 1; subst.
+    + constructor.
+    + constructor 2.
+      * assumption.
+      * apply IHE.
+        eapply remove_var_sound; eassumption.
+Qed.
+
+Lemma linearize_fun_complete {A B} {eq_fun : A -> A -> bool} (E : list (A * B)) :
+  (forall x y, boolSpec (eq_fun x y) (x = y)) ->
+  forall a' b',
+    Lookup E a' b' ->
+    Lookup (linearize_fun eq_fun E) a' b'.
+Proof.
+  intros eq_fun_correct.
+  induction E as [|[? ?]]; simpl.
+  - inversion 1.
+  - inversion 1; subst.
+    + constructor.
+    + constructor 2.
+      * assumption.
+      * eapply remove_var_fun_complete; my_auto.
+Qed.  
+
+Lemma linearize_complete {A B} {eq_dec : DecidableEq A} (E : list (A * B)) :
+  forall a' b',
+    Lookup E a' b' ->
+    Lookup (linearize E) a' b'.
+Proof.
+  induction E as [|[? ?]]; simpl.
+  - inversion 1.
+  - inversion 1; subst.
+    + constructor.
+    + constructor 2.
+      * assumption.
+      * eapply remove_var_complete; my_auto.
+Qed.  
+
+Lemma linear_remove_var_fun {A B} {eq_fun : A -> A -> bool} a (E : list (A * B)) :
+  (forall x y, boolSpec (eq_fun x y) (x = y)) ->
+  linear E -> linear (remove_var_fun eq_fun a E).
+Proof.
+  intros eq_fun_correct.
+  induction E as [|[? ?]]; simpl.
+  - my_auto.
+  - match goal with
+    | [|- context[eq_fun ?a1 ?a2] ] =>
+        generalize (eq_fun_correct a1 a2);
+        destruct (eq_fun a1 a2);
+        simpl; intros ?
+    end.
+    + inversion 1; my_auto.
+    + inversion 1; subst.
+      constructor.
+      * intros ? ?.
+        match goal with
+        | [H : forall _, neg (Lookup E _ _) |- _] =>
+            eapply H;
+            eapply remove_var_fun_sound;
+            eassumption
+        end.
+      * my_auto.
+Qed.
+
+Lemma linear_remove_var {A B} {eq_dec : DecidableEq A} a (E : list (A * B)) :
+  linear E -> linear (remove_var a E).
+Proof.
+  induction E as [|[? ?]]; simpl.
+  - my_auto.
+  - decide_destruct.
+    + inversion 1; my_auto.
+    + inversion 1; subst.
+      constructor.
+      * intros ? ?.
+        match goal with
+        | [H : forall _, neg (Lookup E _ _) |- _] =>
+            eapply H;
+            eapply remove_var_sound;
+            eassumption
+        end.
+      * my_auto.
+Qed.
+
+Lemma linearize_fun_linear {A B} {eq_fun : A -> A -> bool} (E : list (A * B)) :
+  (forall x y, boolSpec (eq_fun x y) (x = y)) ->  
+  linear (linearize_fun eq_fun E).
+Proof.
+  intros eq_fun_correct.
+  induction E as [|[? ?]]; simpl.
+  - constructor.
+  - econstructor.
+    + apply remove_var_fun_Lookup; assumption.
+    + apply linear_remove_var_fun; assumption.
+Qed.
+
+Lemma linearize_linear {A B} {eq_dec : DecidableEq A} (E : list (A * B)) :
+  linear (linearize E).
+Proof.
+  induction E as [|[? ?]]; simpl.
+  - constructor.
+  - econstructor.
+    + apply remove_var_Lookup.
+    + apply linear_remove_var; assumption.
+Qed.
+
+Fixpoint context_linear_all_fun {A B} (eq_fun : A -> A -> bool) (P_fun : A -> B -> bool) E : bool :=
+  match E with
+  | nil           => true
+  | cons (a, b) E => andb (P_fun a b) (context_linear_all_fun eq_fun P_fun E)
+  end.
+
+Fixpoint context_linear_all_fun_correct {A B} {eq_fun : A -> A -> bool} {P_fun : A -> B -> bool} {P : A -> B -> Type} {E} :
+  (forall x y, boolSpec (eq_fun x y) (x = y)) ->
+  (forall x y, boolSpec (P_fun  x y) (P x y)) ->
+  linear E ->
+  boolSpec (context_linear_all_fun eq_fun P_fun E) (forall a b, Lookup E a b -> P a b).
+Proof.
+  intros eq_fun_correct P_fun_correct.
+  induction E as [| [a b] E IH]; simpl.
+  - my_auto.
+  - match goal with
+    | [|- context[P_fun ?a1 ?a2] ] =>
+        generalize (P_fun_correct a1 a2);
+        destruct (P_fun a1 a2);
+        simpl; [intros ?| intros P_neg]
+    end.
+    + inversion 1 as [| ? ? ? Hfalse Hlinear]; subst.
+      match goal with
+      | [|- context[context_linear_all_fun eq_fun P_fun ?E] ] =>
+          generalize (context_linear_all_fun_correct _ _ _ _ _ E eq_fun_correct P_fun_correct Hlinear);
+          destruct (context_linear_all_fun eq_fun P_fun E);
+          simpl; intros ?
+      end.
+      inversion 1; my_auto.
+      intros Hlookup.
+      apply (IH Hlinear); intros.
+      apply Hlookup.
+      constructor 2.
+      * intros ?; subst; firstorder.
+      * assumption.
+    + intros Hlinear Hfalse.
+      apply P_neg.
+      apply Hfalse.
+      constructor.
+Qed.
+
+Definition lookup_linear_dec {A B} {eq_dec : DecidableEq A} {P : A -> B -> Type} (P_dec : forall a b, Decision (P a b)) E :
+  linear E ->
+  Decision (forall a b, Lookup E a b -> P a b).
+Proof.
+  induction E as [| [a b] E IH].
+  - left; inversion 1.
+  - destruct (P_dec a b) as [P_pos | P_neg].
+    + inversion 1 as [| ? ? ? Hfalse Hlinear]; subst.
+      destruct (IH Hlinear) as [IH_pos | IH_neg].
+      * left; inversion 1; subst.
+          assumption.
+          apply IH_pos; assumption.
+      * right; intros H.
+        apply IH_neg; intros.
+        apply H.
+        constructor 2.
+          intros ?; subst; firstorder.
+          assumption.
+    + right.
+      intros Hfalse.
+      apply P_neg.
+      apply Hfalse.
+      constructor.
+Qed.
+
+Definition context_linear_ind {A B} {eq_dec : DecidableEq A} (P : list (A * B) -> Type) :
+  P nil ->
+  (forall a (b : B) E, (forall b, neg (Lookup E a b)) -> linear E -> P (add E a b)) ->
+  forall E, linear E -> P E.
+Proof.
+  intros Hempty Hadd.
+  induction E as [|[? ?]]; simpl.
+  - auto.
+  - inversion 1; subst.
+    apply Hadd; assumption.
+Qed.
+
+Definition context_all_fun {A B} (eq_fun : A -> A -> bool) (P_fun : A -> B -> bool) E : bool :=
+  context_linear_all_fun eq_fun P_fun (linearize_fun eq_fun E).
+
+Lemma context_all_fun_correct {A B} {eq_fun : A -> A -> bool} {P_fun : A -> B -> bool} {P : A -> B -> Type} E :
+  (forall x y, boolSpec (eq_fun x y) (x = y)) ->
+  (forall x y, boolSpec (P_fun  x y) (P x y)) ->
+  boolSpec (context_all_fun eq_fun P_fun E) (forall a b, Lookup E a b -> P a b).
+Proof.
+  intros eq_fun_correct P_fun_correct.
+  do 2 unfold_goal.
+  generalize (context_linear_all_fun_correct eq_fun_correct P_fun_correct (linearize_fun_linear E eq_fun_correct)).
+  destruct (context_linear_all_fun eq_fun P_fun (linearize_fun eq_fun E)); simpl; intros H.
+  - intros.
+    apply H.
+    apply linearize_fun_complete; assumption.
+  - intros Hlookup.
+    apply H; intros.
+    apply Hlookup.
+    eapply linearize_fun_sound; eassumption.
+Qed.
+
+Definition lookup_dec {A B} {eq_dec : DecidableEq A} {P : A -> B -> Type} (P_dec : forall a b, Decision (P a b)) E :
+  Decision (forall a b, Lookup E a b -> P a b).
+Proof.
+  destruct (lookup_linear_dec P_dec (linearize E) (linearize_linear E)) as [Y|N].
+  - left; intros.
+    apply Y.
+    apply linearize_complete.
+    assumption.
+  - right; intros H.
+    apply N; intros.
+    apply H.
+    apply linearize_sound.
+    assumption.
 Qed.
